src/QueryStructure/Implementation/Operations/General/QueryRefinements.v
@@ -1474,63 +1474,63 @@ Defined.
     intros; computes_to_econstructor; computes_to_inv; subst;
       intuition.
     unfold UnIndexedEnsembleListEquivalence in H0; destruct_ex;
-        intuition; subst.
-      apply in_map_iff in H1; destruct_ex; intuition; subst.
-      apply H in H2; intuition.
-      apply H0; eauto.
+      intuition; subst.
+    apply in_map_iff in H1; destruct_ex; intuition; subst.
+    apply H in H2; intuition.
+    apply H0; eauto.
   Qed.
 
 
-Lemma Query_Where_And_Sym {ResultT}
-  : forall (P Q : Prop)
-           (body : Comp (list ResultT)),
-    refine (Query_Where (P /\ Q) body)
-           (Query_Where (Q /\ P) body).
-Proof.
-  intros; rewrite refine_Query_Where_Cond;
-    try reflexivity; intuition.
-Qed.
+  Lemma Query_Where_And_Sym {ResultT}
+    : forall (P Q : Prop)
+             (body : Comp (list ResultT)),
+      refine (Query_Where (P /\ Q) body)
+             (Query_Where (Q /\ P) body).
+  Proof.
+    intros; rewrite refine_Query_Where_Cond;
+      try reflexivity; intuition.
+  Qed.
 
-Lemma flatten_CompList_Prop {A}
-  : forall (P : Ensemble A) (P_dec : DecideableEnsemble P) (As As' : list A),
-    FlattenCompList.flatten_CompList (map (fun a : A => Query_Where (P a)
-                                                                    (Query_Return a) ) As) ↝ As'
-    -> forall a, List.In a As' -> P a.
-Proof.
-  induction As; simpl; intros; computes_to_inv; subst; simpl in *; intuition.
-  unfold Query_Where, Query_Return in H; computes_to_inv; intuition.
-  destruct (dec a) eqn: ?.
-  - rewrite dec_decides_P in Heqb.
-    pose proof (H1 Heqb); computes_to_inv;
-      subst; simpl in *; subst; intuition eauto.
-    subst; eauto.
-  - apply Decides_false in Heqb; apply H2 in Heqb; subst; simpl in *;
-      eauto.
-Qed.
+  Lemma flatten_CompList_Prop {A}
+    : forall (P : Ensemble A) (P_dec : DecideableEnsemble P) (As As' : list A),
+      FlattenCompList.flatten_CompList (map (fun a : A => Query_Where (P a)
+                                                                      (Query_Return a) ) As) ↝ As'
+      -> forall a, List.In a As' -> P a.
+  Proof.
+    induction As; simpl; intros; computes_to_inv; subst; simpl in *; intuition.
+    unfold Query_Where, Query_Return in H; computes_to_inv; intuition.
+    destruct (dec a) eqn: ?.
+    - rewrite dec_decides_P in Heqb.
+      pose proof (H1 Heqb); computes_to_inv;
+        subst; simpl in *; subst; intuition eauto.
+      subst; eauto.
+    - apply Decides_false in Heqb; apply H2 in Heqb; subst; simpl in *;
+        eauto.
+  Qed.
 
-Lemma flatten_CompList_Subset {A}
-  : forall (P : Ensemble A) (P_dec : DecideableEnsemble P) (As As' : list A),
-    FlattenCompList.flatten_CompList (map (fun a : A => Query_Where (P a)
-                                                                    (Query_Return a) ) As) ↝ As'
-    -> forall a, List.In a As' -> List.In a As.
-Proof.
-  induction As; simpl; intros; computes_to_inv; subst; simpl in *; intuition.
-  unfold Query_Where, Query_Return in H; computes_to_inv; intuition.
-  destruct (dec a) eqn: ?.
-  - rewrite dec_decides_P in Heqb.
-    pose proof (H1 Heqb); computes_to_inv;
-      subst; simpl in *; subst; intuition eauto.
-  - apply Decides_false in Heqb; apply H2 in Heqb; subst; simpl in *;
-      eauto.
-Qed.
+  Lemma flatten_CompList_Subset {A}
+    : forall (P : Ensemble A) (P_dec : DecideableEnsemble P) (As As' : list A),
+      FlattenCompList.flatten_CompList (map (fun a : A => Query_Where (P a)
+                                                                      (Query_Return a) ) As) ↝ As'
+      -> forall a, List.In a As' -> List.In a As.
+  Proof.
+    induction As; simpl; intros; computes_to_inv; subst; simpl in *; intuition.
+    unfold Query_Where, Query_Return in H; computes_to_inv; intuition.
+    destruct (dec a) eqn: ?.
+    - rewrite dec_decides_P in Heqb.
+      pose proof (H1 Heqb); computes_to_inv;
+        subst; simpl in *; subst; intuition eauto.
+    - apply Decides_false in Heqb; apply H2 in Heqb; subst; simpl in *;
+        eauto.
+  Qed.
 
-Lemma flatten_CompList_nil {A}
-  : forall (P : Ensemble A) (P_dec : DecideableEnsemble P) (As : list A),
-    FlattenCompList.flatten_CompList
-      (map (fun a : A => Query_Where (P a)
-                               (Query_Return a)) As) ↝ nil
-    -> forall a, List.In a As -> ~ P a.
-Proof.
+  Lemma flatten_CompList_nil {A}
+    : forall (P : Ensemble A) (P_dec : DecideableEnsemble P) (As : list A),
+      FlattenCompList.flatten_CompList
+        (map (fun a : A => Query_Where (P a)
+                                       (Query_Return a)) As) ↝ nil
+      -> forall a, List.In a As -> ~ P a.
+  Proof.
     induction As; simpl; intros; computes_to_inv; subst; simpl in *; intuition.
     unfold Query_Where, Query_Return in H; computes_to_inv; intuition.
     destruct (dec a) eqn: ?.
@@ -1543,34 +1543,61 @@ Proof.
       discriminate.
     - eapply IHAs; eauto.
       apply app_eq_nil in H''; intuition; subst; eauto.
-Qed.
+  Qed.
 
-Corollary For_In_Where_Prop {qs_schema}
-  : forall idx r_o P l,
-    DecideableEnsemble P
-    -> Query_For (Query_In (qs_schema := qs_schema)
-                     r_o idx (fun r : RawTuple => Query_Where (P r)
-                                                        (Query_Return r) )) ↝ l
-    -> Forall P l.
-Proof.
-  unfold Query_In, Query_For, QueryResultComp; intros; computes_to_inv.
-  apply Forall_forall; intros.
-  eapply flatten_CompList_Prop in H'0; eauto.
-  symmetry in H'.
-  eapply Permutation_in; eauto.
-Qed.
+  Corollary For_In_Where_Prop {qs_schema}
+    : forall idx r_o P l,
+      DecideableEnsemble P
+      -> Query_For (Query_In (qs_schema := qs_schema)
+                             r_o idx (fun r : RawTuple => Query_Where (P r)
+                                                                      (Query_Return r) )) ↝ l
+      -> Forall P l.
+  Proof.
+    unfold Query_In, Query_For, QueryResultComp; intros; computes_to_inv.
+    apply Forall_forall; intros.
+    eapply flatten_CompList_Prop in H'0; eauto.
+    symmetry in H'.
+    eapply Permutation_in; eauto.
+  Qed.
 
-Corollary For_UnConstrQuery_In_Where_Prop {qs_schema}
-  : forall idx r_o P l,
-    DecideableEnsemble P
-    -> Query_For (UnConstrQuery_In (qsSchema := qs_schema)
-                     r_o idx (fun r : RawTuple => Query_Where (P r)
-                                                        (Query_Return r) )) ↝ l
-    -> Forall P l.
-Proof.
-  unfold UnConstrQuery_In, Query_For, QueryResultComp; intros; computes_to_inv.
-  apply Forall_forall; intros.
-  eapply flatten_CompList_Prop in H'0; eauto.
-  symmetry in H'.
-  eapply Permutation_in; eauto.
-Qed.
+  Corollary For_UnConstrQuery_In_Where_Prop {qs_schema}
+    : forall idx r_o P l,
+      DecideableEnsemble P
+      -> Query_For (UnConstrQuery_In (qsSchema := qs_schema)
+                                     r_o idx (fun r : RawTuple => Query_Where (P r)
+                                                                              (Query_Return r) )) ↝ l
+      -> Forall P l.
+  Proof.
+    unfold UnConstrQuery_In, Query_For, QueryResultComp; intros; computes_to_inv.
+    apply Forall_forall; intros.
+    eapply flatten_CompList_Prop in H'0; eauto.
+    symmetry in H'.
+    eapply Permutation_in; eauto.
+  Qed.
+
+  Lemma refine_For_Map {resultT resultT'}
+    : forall comp
+             (f : resultT' -> resultT),
+      refine (Query_For (results <- comp; ret (map f results)))
+             (results <- Query_For comp; ret (map f results)).
+  Proof.
+    intros; unfold Query_For; autorewrite with monad laws.
+    f_equiv; intro.
+    intros ? ?; computes_to_inv; subst.
+    computes_to_econstructor; rewrite Permutation_map; eauto.
+  Qed.
+
+  Corollary refine_UnConstrQuery_In_Query_Where_Cond
+            {qs_schema}
+    : forall (r_n : UnConstrQueryStructure qs_schema)
+             Ridx
+             (ResultT : Type)
+             (P Q : _ -> Prop)
+             (body : _ -> Comp (list ResultT)),
+      (forall tup, P tup <-> Q tup) ->
+      refine (UnConstrQuery_In r_n Ridx (fun tup => Query_Where (P tup) (body tup)))
+             (UnConstrQuery_In r_n Ridx (fun tup => Query_Where (Q tup) (body tup))).
+  Proof.
+    intros; apply refine_UnConstrQuery_In; intro.
+    apply refine_Query_Where_Cond; eauto.
+  Qed.
